add fib32 proof, still a few sorry

Clean/Tables/Fibonacci32.lean
@@ -6,17 +6,6 @@ import Clean.Gadgets.Equality.U32
 import Clean.Types.U32
 
 
-/-
-  8-bit Fibonacci inductive table definition. The i-th row of the table
-  contains the values of the Fibonacci sequence at i and i+1, modulo 256.
-
-  0        | 1
-  ...
-  fib(i)   | fib(i+1)
-  fib(i+1) | fib(i+2)
-  ...
-
--/
 namespace Tables.Fibonacci32
 variable {p : ℕ}
 variable [p_large_enough: Fact (p > 2*2^32)]
@@ -24,27 +13,32 @@ variable [p_large_enough: Fact (p > 2*2^32)]
 lemma p_large_enough' : Fact (p > 512) := by
   apply Fact.mk; linarith [p_large_enough.elim]
 
-variable [Fact (p ≠ 0)] [Fact p.Prime]
+variable [Fact p.Prime]
+
+structure RowType (F : Type) where
+  x: U32 F
+  y: U32 F
+
+instance (F : Type) : StructuredElements RowType F where
+  size := 8
+  to_elements s := vec [s.x.x0, s.x.x1, s.x.x2, s.x.x3, s.y.x0, s.y.x1, s.y.x2, s.y.x3]
+  from_elements v :=
+    -- TODO is it possible to define in terms of StructuredElements.from_elements of the U32?
+    let ⟨ [x0, x1, x2, x3, y0, y1, y2, y3], _ ⟩ := v
+    ⟨ ⟨ x0, x1, x2, x3 ⟩, ⟨ y0, y1, y2, y3 ⟩ ⟩
 
 /--
   inductive contraints that are applied every two rows of the trace.
 -/
-def recursive_relation : TwoRowsConstraint (F p) 8 := do
-  let x0 <- TableConstraint.get_cell (CellOffset.curr 0)
-  let x1 <- TableConstraint.get_cell (CellOffset.curr 1)
-  let x2 <- TableConstraint.get_cell (CellOffset.curr 2)
-  let x3 <- TableConstraint.get_cell (CellOffset.curr 3)
+def recursive_relation : TwoRowsConstraint RowType (F p) := do
+  let curr : RowType _ := StructuredElements.from_elements (<-TableConstraint.get_curr_row)
+  let next : RowType _ := StructuredElements.from_elements (<-TableConstraint.get_next_row)
 
-  let y0 <- TableConstraint.get_cell (CellOffset.curr 4)
-  let y1 <- TableConstraint.get_cell (CellOffset.curr 5)
-  let y2 <- TableConstraint.get_cell (CellOffset.curr 6)
-  let y3 <- TableConstraint.get_cell (CellOffset.curr 7)
-
-  let x : U32 (Expression (F p)) := ⟨x0, x1, x2, x3⟩
-  let y : U32 (Expression (F p)) := ⟨y0, y1, y2, y3⟩
-
-
-  let z <- TableConstraint.subcircuit Gadgets.Addition32Full.circuit {x, y, carry_in:=0}
+  let z <- TableConstraint.subcircuit Gadgets.Addition32Full.circuit {
+    x := curr.x,
+    y := curr.y,
+    carry_in:=0
+  }
 
   if let ⟨⟨var z0, var z1, var z2, var z3⟩, _⟩ := z then
     TableConstraint.assign z0 (CellOffset.next 4)
@@ -52,53 +46,35 @@ def recursive_relation : TwoRowsConstraint (F p) 8 := do
     TableConstraint.assign z2 (CellOffset.next 6)
     TableConstraint.assign z3 (CellOffset.next 7)
 
-  let x0_next <- TableConstraint.get_cell (CellOffset.next 0)
-  let x1_next <- TableConstraint.get_cell (CellOffset.next 1)
-  let x2_next <- TableConstraint.get_cell (CellOffset.next 2)
-  let x3_next <- TableConstraint.get_cell (CellOffset.next 3)
-
-  let x_next : U32 (Expression (F p)) := ⟨x0_next, x1_next, x2_next, x3_next⟩
-  TableConstraint.assertion Gadgets.Equality.U32.circuit ⟨y, x_next⟩
+  TableConstraint.assertion Gadgets.Equality.U32.circuit ⟨curr.y, next.x⟩
 
 /--
   boundary constraints that are applied at the beginning of the trace.
   This is our "base case" for the Fibonacci sequence.
 -/
-def boundary : SingleRowConstraint (F p) 8 := do
-  let x0 <- TableConstraint.get_cell (CellOffset.curr 0)
-  let x1 <- TableConstraint.get_cell (CellOffset.curr 1)
-  let x2 <- TableConstraint.get_cell (CellOffset.curr 2)
-  let x3 <- TableConstraint.get_cell (CellOffset.curr 3)
-  let y0 <- TableConstraint.get_cell (CellOffset.curr 4)
-  let y1 <- TableConstraint.get_cell (CellOffset.curr 5)
-  let y2 <- TableConstraint.get_cell (CellOffset.curr 6)
-  let y3 <- TableConstraint.get_cell (CellOffset.curr 7)
+def boundary : SingleRowConstraint RowType (F p) := do
+  let row : RowType _ := StructuredElements.from_elements (<-TableConstraint.get_curr_row)
 
-  let x : U32 (Expression (F p)) := ⟨x0, x1, x2, x3⟩
-  let y : U32 (Expression (F p)) := ⟨y0, y1, y2, y3⟩
+  TableConstraint.assertion Gadgets.Equality.U32.circuit ⟨row.x, ⟨0, 0, 0, 0⟩⟩
+  TableConstraint.assertion Gadgets.Equality.U32.circuit ⟨row.y, ⟨1, 0, 0, 0⟩⟩
 
-  TableConstraint.assertion Gadgets.Equality.U32.circuit ⟨x, U32.decompose_nat_expr 0⟩
-  TableConstraint.assertion Gadgets.Equality.U32.circuit ⟨y, U32.decompose_nat_expr 1⟩
-
-def fib32_table : List (TableOperation (F p) 8) := [
+def fib32_table : List (TableOperation RowType (F p)) := [
   TableOperation.Boundary 0 boundary,
   TableOperation.EveryRowExceptLast recursive_relation,
 ]
 
-def assumptions {N : ℕ} (trace : TraceOfLength (F p) 8 N) : Prop :=
+def assumptions {N : ℕ} (trace : TraceOfLength (F p) RowType N) : Prop :=
   N > 2 ∧
-  trace.forAllRowsOfTrace (fun row => (row 1).val < 256)
+  trace.forAllRowsOfTrace (fun row => (row.y).is_normalized)
 
 def fib32 : ℕ -> ℕ
   | 0 => 0
   | 1 => 1
   | (n + 2) => (fib32 n + fib32 (n + 1)) % 2^32
 
-def spec {N : ℕ} (trace : TraceOfLength (F p) 8 N) : Prop :=
+def spec {N : ℕ} (trace : TraceOfLength (F p) RowType N) : Prop :=
   trace.forAllRowsOfTraceWithIndex (λ row index =>
-    let x := (U32.mk (row 0) (row 1) (row 2) (row 3)).value
-    let y := (U32.mk (row 4) (row 5) (row 6) (row 7)).value
-    (x = fib32 index) ∧ (y = fib32 (index + 1))
+    (row.x.value = fib32 index) ∧ (row.y.value = fib32 (index + 1))
     )
 
 
@@ -107,13 +83,199 @@ lemma fib32_less_than_2_32 (n : ℕ) : fib32 n < 2^32 := by
   repeat {simp [fib32]}; apply Nat.mod_lt; simp
 
 
-def formal_fib32_table : FormalTable (F:=(F p)) := {
-  M := 8,
+def boundary_var1 : ((boundary (p:=p) { offset := 0, assignment := fun _ ↦ { rowOffset := 0, column := 0 } }).1.1.2 0) = CellOffset.curr 0
+  := by simp [boundary, bind, table_norm]; rfl
+def boundary_var2 : ((boundary (p:=p) { offset := 0, assignment := fun _ ↦ { rowOffset := 0, column := 0 } }).1.1.2 1) = CellOffset.curr 1
+  := by simp [boundary, bind, table_norm]; rfl
+def boundary_var3 : ((boundary (p:=p) { offset := 0, assignment := fun _ ↦ { rowOffset := 0, column := 0 } }).1.1.2 2) = CellOffset.curr 2
+  := by simp [boundary, bind, table_norm]; rfl
+def boundary_var4 : ((boundary (p:=p) { offset := 0, assignment := fun _ ↦ { rowOffset := 0, column := 0 } }).1.1.2 3) = CellOffset.curr 3
+  := by simp [boundary, bind, table_norm]; rfl
+def boundary_var5 : ((boundary (p:=p) { offset := 0, assignment := fun _ ↦ { rowOffset := 0, column := 0 } }).1.1.2 4) = CellOffset.curr 4
+  := by simp [boundary, bind, table_norm]; rfl
+def boundary_var6 : ((boundary (p:=p) { offset := 0, assignment := fun _ ↦ { rowOffset := 0, column := 0 } }).1.1.2 5) = CellOffset.curr 5
+  := by simp [boundary, bind, table_norm]; rfl
+def boundary_var7 : ((boundary (p:=p) { offset := 0, assignment := fun _ ↦ { rowOffset := 0, column := 0 } }).1.1.2 6) = CellOffset.curr 6
+  := by simp [boundary, bind, table_norm]; rfl
+def boundary_var8 : ((boundary (p:=p) { offset := 0, assignment := fun _ ↦ { rowOffset := 0, column := 0 } }).1.1.2 7) = CellOffset.curr 7
+  := by simp [boundary, bind, table_norm]; rfl
+
+def rec_var0 : ((recursive_relation (p:=p) { offset := 0, assignment := fun _ ↦ { rowOffset := 0, column := 0 } }).1.1.2 0) = CellOffset.curr 0
+  := by simp [recursive_relation, bind, table_norm]; rfl
+def rec_var1 : ((recursive_relation (p:=p) { offset := 0, assignment := fun _ ↦ { rowOffset := 0, column := 0 } }).1.1.2 1) = CellOffset.curr 1
+  := by simp [recursive_relation, bind, table_norm]; rfl
+def rec_var2 : ((recursive_relation (p:=p) { offset := 0, assignment := fun _ ↦ { rowOffset := 0, column := 0 } }).1.1.2 2) = CellOffset.curr 2
+  := by simp [recursive_relation, bind, table_norm]; rfl
+def rec_var3 : ((recursive_relation (p:=p) { offset := 0, assignment := fun _ ↦ { rowOffset := 0, column := 0 } }).1.1.2 3) = CellOffset.curr 3
+  := by simp [recursive_relation, bind, table_norm]; rfl
+def rec_var4 : ((recursive_relation (p:=p) { offset := 0, assignment := fun _ ↦ { rowOffset := 0, column := 0 } }).1.1.2 4) = CellOffset.curr 4
+  := by simp [recursive_relation, bind, table_norm]; rfl
+def rec_var5 : ((recursive_relation (p:=p) { offset := 0, assignment := fun _ ↦ { rowOffset := 0, column := 0 } }).1.1.2 5) = CellOffset.curr 5
+  := by simp [recursive_relation, bind, table_norm]; rfl
+def rec_var6 : ((recursive_relation (p:=p) { offset := 0, assignment := fun _ ↦ { rowOffset := 0, column := 0 } }).1.1.2 6) = CellOffset.curr 6
+  := by simp [recursive_relation, bind, table_norm]; rfl
+def rec_var7 : ((recursive_relation (p:=p) { offset := 0, assignment := fun _ ↦ { rowOffset := 0, column := 0 } }).1.1.2 7) = CellOffset.curr 7
+  := by simp [recursive_relation, bind, table_norm]; rfl
+
+def rec_var8 : ((recursive_relation (p:=p) { offset := 0, assignment := fun _ ↦ { rowOffset := 0, column := 0 } }).1.1.2 8) = CellOffset.next 8
+  := by simp [recursive_relation, bind, table_norm]; rfl
+
+
+def rec_var16 : ((recursive_relation (p:=p) { offset := 0, assignment := fun _ ↦ { rowOffset := 0, column := 0 } }).1.1.2 16) = CellOffset.next 4
+  := by simp [recursive_relation, bind, table_norm]; rfl
+def rec_var18 : ((recursive_relation (p:=p) { offset := 0, assignment := fun _ ↦ { rowOffset := 0, column := 0 } }).1.1.2 18) = CellOffset.next 5
+  := by simp [recursive_relation, bind, table_norm]; rfl
+def rec_var20 : ((recursive_relation (p:=p) { offset := 0, assignment := fun _ ↦ { rowOffset := 0, column := 0 } }).1.1.2 20) = CellOffset.next 6
+  := by simp [recursive_relation, bind, table_norm]; rfl
+def rec_var22 : ((recursive_relation (p:=p) { offset := 0, assignment := fun _ ↦ { rowOffset := 0, column := 0 } }).1.1.2 22) = CellOffset.next 7
+  := by simp [recursive_relation, bind, table_norm]; rfl
+
+lemma lift_rec_add (curr : Row (F p) RowType) (next : Row (F p) RowType)
+  : TableConstraint.constraints_hold_on_window recursive_relation ⟨<+> +> curr +> next, by simp [Trace.len]⟩ ->
+  (curr.x.is_normalized -> curr.y.is_normalized -> next.y.value = (curr.x.value + curr.y.value) % 2^32) := by
+
+  simp [table_norm, StructuredElements.size, StructuredElements.from_elements]
+  intros h_add h_eq
+
+  -- TODO: ok this is very annoying
+  -- why can't simp figure out those relations?
+  rw [
+    show ((3 : Fin 4).val % 6 % 7 % 8) = 3 by rfl,
+    show ((4 : Fin 5).val % 7 % 8) = 4 by rfl,
+    show (((5 : Fin 6).val % 8)) = 5 by rfl,
+    show ((6 : Fin 7).val) = 6 by rfl,
+    show (7 : Fin 8).val = 7 by rfl,
+  ] at h_add
+
+  simp [Circuit.subcircuit_soundness] at h_add
+  simp only [rec_var0, rec_var1, rec_var2, rec_var3, rec_var4, rec_var5, rec_var6, rec_var7] at h_add
+  simp [CellOffset.curr, Gadgets.Addition32Full.circuit, Gadgets.Addition32Full.spec,
+    table_norm, StructuredElements.to_elements, from_values] at h_add
+  simp [to_vars, circuit_norm, table_norm] at h_add
+
+  simp [rec_var16, rec_var18, rec_var20, rec_var22] at h_add
+  simp [CellOffset.next] at h_add
+  simp [
+    show (3 : Fin 8).val = 3 by rfl,
+    show (4 : Fin 8).val = 4 by rfl,
+    show (5 : Fin 8).val = 5 by rfl,
+    show (6 : Fin 8).val = 6 by rfl,
+    show (7 : Fin 8).val = 7 by rfl,
+  ] at h_add
+  simp [Gadgets.Addition32Full.assumptions] at h_add
+
+  intro h_norm_x h_norm_y
+  specialize h_add h_norm_x h_norm_y
+  simp only [h_add]
+
+
+lemma lift_rec_eq (curr : Row (F p) RowType) (next : Row (F p) RowType)
+  : TableConstraint.constraints_hold_on_window recursive_relation ⟨<+> +> curr +> next, by simp [Trace.len]⟩ ->
+  curr.y = next.x := by
+
+  simp [table_norm, StructuredElements.size, StructuredElements.from_elements]
+  intros _ h_eq
+
+  -- TODO: ok this is very annoying
+  -- why can't simp figure out those relations?
+  rw [
+    show ((3 : Fin 4).val % 6 % 7 % 8) = 3 by rfl,
+    show ((4 : Fin 5).val % 7 % 8) = 4 by rfl,
+    show (((5 : Fin 6).val % 8)) = 5 by rfl,
+    show ((6 : Fin 7).val) = 6 by rfl,
+    show (7 : Fin 8).val = 7 by rfl,
+  ] at h_eq
+
+  simp [Circuit.formal_assertion_to_subcircuit, Circuit.subassertion_soundness, from_values, Gadgets.Equality.U32.circuit, to_vars] at h_eq
+  simp only [rec_var5, rec_var6, rec_var7, rec_var8] at h_eq
+  simp [CellOffset.curr, Gadgets.Addition32Full.circuit, Gadgets.Addition32Full.spec,
+    table_norm, StructuredElements.to_elements, from_values, Gadgets.Equality.U32.spec] at h_eq
+
+  simp [
+    show (3 : Fin 8).val = 3 by rfl,
+    show (4 : Fin 8).val = 4 by rfl,
+    show (5 : Fin 8).val = 5 by rfl,
+    show (6 : Fin 8).val = 6 by rfl,
+    show (7 : Fin 8).val = 7 by rfl,
+  ] at h_eq
+
+  sorry
+
+
+def formal_fib32_table : FormalTable (F p) RowType := {
   constraints := fib32_table,
   assumptions := assumptions,
   spec := spec,
   soundness := by
-    sorry
+    intro N trace
+    simp only [assumptions, gt_iff_lt, Fin.isValue, and_imp, Fin.isValue, fib32_table, spec]
+    rw [TraceOfLength.forAllRowsOfTraceWithIndex, TraceOfLength.forAllRowsOfTrace, table_constraints_hold]
+
+
+    intro _N_assumption
+
+    induction' trace.val using Trace.everyRowTwoRowsInduction with first_row curr next rest _ ih2
+    · simp [table_norm]
+    · intro _
+      simp only [table_norm]
+      simp [table_norm, Circuit.formal_assertion_to_subcircuit, Circuit.subassertion_soundness, circuit_norm]
+
+      rw [
+        show ((3 : Fin 4).val % 6 % 7 % 8) = 3 by rfl,
+        show ((4 : Fin 5).val % 7 % 8) = 4 by rfl,
+        show (((5 : Fin 6).val % 8)) = 5 by rfl,
+        show ((6 : Fin 7).val) = 6 by rfl,
+        show (7 : Fin 8).val = 7 by rfl,
+      ]
+
+      simp only [boundary_var1, boundary_var2, boundary_var3, boundary_var4, boundary_var5, boundary_var6, boundary_var7, boundary_var8]
+      simp [CellOffset.curr, Gadgets.Equality.U32.circuit, Gadgets.Equality.U32.spec]
+
+      simp [
+        show (3 : Fin 8).val = 3 by rfl,
+        show (4 : Fin 8).val = 4 by rfl,
+        show (5 : Fin 8).val = 5 by rfl,
+        show (6 : Fin 8).val = 6 by rfl,
+        show (7 : Fin 8).val = 7 by rfl,
+      ]
+      intros b0 b1 b2 b3 b4 b5 b6 b7
+
+      simp only [U32.value, fib32]
+      rw [b0, b1, b2, b3, b4, b5, b6, b7]
+      simp [ZMod.val_one]
+
+    · intro lookup_h
+      simp only [TraceOfLength.forAllRowsOfTrace.inner, Fin.isValue] at lookup_h
+
+      -- first of all, we prove the inductive part of the spec
+      unfold TraceOfLength.forAllRowsOfTraceWithIndex.inner
+      intros constraints_hold
+      specialize ih2 lookup_h.right
+
+      unfold table_constraints_hold.foldl at constraints_hold
+      simp only [Trace.len, Nat.succ_ne_zero, ite_false] at constraints_hold
+      unfold table_constraints_hold.foldl at constraints_hold
+      unfold table_constraints_hold.foldl at constraints_hold
+      simp only at constraints_hold
+      specialize ih2 constraints_hold.right
+      simp only [ih2, and_self]
+
+      simp only [Fin.isValue, and_true] at ih2
+      let ⟨curr_fib0, curr_fib1⟩ := ih2.left
+
+      simp only [and_true]
+
+      have add_spec := lift_rec_add curr next constraints_hold.left
+      have eq_spec := lift_rec_eq curr next constraints_hold.left
+
+      have h_lookup_first : curr.x.is_normalized := by
+        -- TODO: should be easy
+        sorry
+
+      specialize add_spec h_lookup_first lookup_h.right.left
+      simp [fib32]
+      rw [←curr_fib0, ←curr_fib1, ←eq_spec]
+      simp [add_spec, curr_fib1, Trace.len]
 }
 
 end Tables.Fibonacci32
